Moved modalities to their own file.

coq/Corps/Syntax.v
@@ -8,11 +8,17 @@ From Stdlib Require Import Logic.Eqdep_dec.
 From Stdlib Require Import Program.Equality.
 From Stdlib Require Import Program.Wf.
 
+Require Import Modalities.
+
 Set Implicit Arguments.
 Section CorpsSyntax.
 
   Context {PName : Type} `{EqBool PName}.
-  
+  #[local] Notation mod := (@mod PName).
+  #[local] Definition ptm := @proc_to_mod PName.
+  #[local] Definition PrefixOfT := @PrefixOfT PName.
+  Coercion ptm : PName >-> mod.
+
   Section CorpsTypes.
 
     Inductive type : Type :=
@@ -46,657 +52,6 @@ Section CorpsSyntax.
     Defined.
 
   End CorpsTypes.
-
-  Section Modality.
-
-    Inductive mod : Type :=
-    | base : mod
-    | cons (m : mod) (p : PName) : mod.
-
-    Fixpoint mod2list (m : mod) : list PName :=
-      match m with
-      | base => []
-      | cons m p => (mod2list m) ++ [p]
-      end.
-
-    Lemma mod2list_inj : forall (m1 m2 : mod) , mod2list m1 = mod2list m2 -> m1 = m2.
-    Proof using.
-      intro m1; induction m1; intros m2 eq; destruct m2; cbn in eq; subst; auto.
-      - destruct (app_eq_nil _ _ ltac:(symmetry; exact eq)) as [H0 H1]; inversion H1.
-      - destruct (app_eq_nil _ _ eq) as [H0 H1]; inversion H1.
-      - apply app_inj_tail in eq; destruct eq; subst.
-        apply IHm1 in H0; subst; reflexivity.
-    Qed.        
-
-    Fixpoint mod_eqb (m1 m2 : mod) : bool :=
-      match m1, m2 with
-      | base, base => true
-      | cons m1 p, cons m2 q => eqb p q && mod_eqb m1 m2
-      | _, _ => false
-      end.
-    #[global] Program Instance ModEqB : EqBool mod :=
-      {
-        eqb := mod_eqb
-      }.
-    Next Obligation.
-      revert y H0; solve_eqb_liebniz x.
-    Defined.
-    Next Obligation.
-      solve_eqb_refl.
-    Defined.
-
-    Fixpoint mod_size (m : mod) : nat :=
-      match m with
-      | base => 0
-      | cons m _ => S (mod_size m)
-      end.
-
-    Lemma mod_size_list_length : forall m : mod, mod_size m = length (mod2list m).
-    Proof using.
-      intros m; induction m; cbn; auto.
-      rewrite length_app; cbn.
-      rewrite PeanoNat.Nat.add_1_r.
-      f_equal; exact IHm.
-    Qed.
-
-    Lemma mod_size_zero_to_base : forall m, mod_size m = 0 -> m = base.
-    Proof using.
-      intro m; destruct m; cbn; intro eq; [reflexivity | inversion eq].
-    Qed.
-
-    Fixpoint mod_app (m1 m2 : mod) : mod :=
-      match m2 with
-      | base => m1
-      | cons m2 p => cons (mod_app m1 m2) p
-      end.
-
-    Lemma mod_app2list : forall (m1 m2 : mod), mod2list (mod_app m1 m2) = (mod2list m1) ++ (mod2list m2).
-    Proof using.
-      intros m1 m2; revert m1; induction m2; intro m1; cbn.
-      - symmetry; apply app_nil_r.
-      - rewrite app_assoc; f_equal. apply IHm2.
-    Qed.
-
-
-    Lemma mod_app_assoc : forall m1 m2 m3, mod_app (mod_app m1 m2) m3 = mod_app m1 (mod_app m2 m3).
-    Proof using.
-      intros m1 m2 m3; revert m1 m2; induction m3 as [| m3' IHm3' p]; intros m1 m2; cbn.
-      - reflexivity.
-      - f_equal; apply IHm3'.
-    Qed.
-
-    Lemma mod_app_base : forall m, mod_app m base = m. Proof using. intros m; reflexivity. Qed.
-
-    Lemma mod_base_app : forall m, mod_app base m = m.
-    Proof using.
-      intro m; induction m; cbn; [|rewrite IHm]; reflexivity.
-    Qed.
-
-    Lemma mod_app_size : forall m1 m2, mod_size (mod_app m1 m2) = mod_size m1 + mod_size m2.
-    Proof using.
-      intros m1 m2; revert m1; induction m2 as [| m2' IHm2' p]; intro m1; cbn;
-        [|rewrite IHm2']; lia.
-    Qed.
-
-    Lemma mod_app_id_inv : forall m1 m2, m1 = mod_app m1 m2 -> m2 = base.
-    Proof using.
-      intros m1 m2 eq.
-      apply mod_size_zero_to_base.
-      apply (f_equal mod_size) in eq; rewrite mod_app_size in eq.
-      lia.
-    Qed.
-
-    Lemma mod_app_base_inv : forall m1 m2, mod_app m1 m2 = base -> m1 = base /\ m2 = base.
-    Proof using.
-      intros m1 m2 eq; destruct m1; destruct m2; try (inversion eq; fail); split; reflexivity.
-    Qed.
-
-    Definition proc_to_mod (p : PName) : mod := cons base p.
-
-    Lemma proc_to_mod_inj : forall p q, proc_to_mod p = proc_to_mod q -> p = q.
-    Proof using.
-      intros p q H0; unfold proc_to_mod in H0; inversion H0; reflexivity.
-    Qed.
-
-    #[global] Coercion proc_to_mod : PName >-> mod.
-
-    Lemma mod_app_first_inj : forall (p q : PName) (m1 m2 : mod),
-        mod_app p m1 = mod_app q m2 ->
-        p = q /\ m1 = m2.
-    Proof using.
-      intros p q m1; revert p q; induction m1; cbn; intros q r m2 eq.
-      destruct m2; inversion eq; subst; auto.
-      symmetry in H1; apply mod_app_base_inv in H1; destruct H1; subst; auto.
-      inversion H0.
-      destruct m2; inversion eq; subst; auto.
-      apply mod_app_base_inv in H1; destruct H1; subst; auto.
-      inversion H0.
-      apply IHm1 in H1; destruct H1; subst; auto.
-    Qed.
-
-    Fixpoint list2mod (l : list PName) : mod :=
-      match l with
-      | [] => base
-      | p :: l' => mod_app p (list2mod l')
-      end.
-
-    Lemma list2mod_inj : forall (l1 l2 : list PName), list2mod l1 = list2mod l2 -> l1 = l2.
-    Proof using.
-      intro l1; induction l1; intros l2 eq; cbn in *.
-      - destruct l2; cbn in eq; auto;
-          symmetry in eq; apply mod_app_base_inv in eq; destruct eq as [eq0 eq1]; inversion eq0.
-      - destruct l2; cbn in eq; auto.
-        -- apply mod_app_base_inv in eq; destruct eq as [eq0 eq1]; inversion eq0.
-        -- apply mod_app_first_inj in eq; destruct eq; subst; auto.
-           apply IHl1 in H1; subst; reflexivity.
-    Qed.
-
-    Lemma list2mod2list : forall (l : list PName),
-        mod2list (list2mod l) = l.
-    Proof using.
-      intro l; induction l; cbn; auto.
-      rewrite mod_app2list; cbn. f_equal; exact IHl.
-    Qed.
-
-    Lemma app2mod_app : forall (l1 l2 : list PName),
-        list2mod (l1 ++ l2) = mod_app (list2mod l1) (list2mod l2).
-    Proof using.
-      intro l1; induction l1; cbn; intro l2.
-      rewrite mod_base_app; reflexivity.
-      rewrite IHl1. symmetry; apply mod_app_assoc.
-    Qed.
-    
-    Lemma mod2list2mod : forall (m : mod),
-        list2mod (mod2list m) = m.
-    Proof using.
-      intro m; induction m; cbn; auto.
-      rewrite app2mod_app; cbn. f_equal; exact IHm.
-    Qed.
-
-    Inductive SuffixOf : mod -> mod -> Prop :=
-    | SO_base (m : mod) : SuffixOf base m
-    | SO_step {m1 m2 : mod} (sfx : SuffixOf m1 m2) (p : PName)
-      : SuffixOf (cons m1 p) (cons m2 p).
-
-    Fixpoint SO_refl (m : mod) : SuffixOf m m :=
-      match m with
-      | base => SO_base base
-      | cons m' p => SO_step (SO_refl m') p
-      end.
-
-    #[global] Instance SuffixOfRefl : Reflexive SuffixOf := SO_refl.
-
-    Lemma suffix_has_prefix : forall m1 m2, SuffixOf m1 m2 -> exists m3, mod_app m3 m1 = m2.
-    Proof using.
-      intros m1 m2 sfx; induction sfx; cbn.
-      - exists m; reflexivity.
-      - destruct IHsfx as [m3 eq]; exists m3; rewrite eq; reflexivity.
-    Qed.
-
-    Lemma suffix_of_prefixed : forall m1 m2, SuffixOf m2 (mod_app m1 m2).
-    Proof using.
-      intros m1 m2; revert m1; induction m2; intro m1; cbn.
-      - apply SO_base.
-      - apply SO_step. apply IHm2.
-    Qed.
-
-    Lemma has_prefix_is_suffix : forall m1 m2 m3, mod_app m3 m1 = m2 -> SuffixOf m1 m2.
-    Proof using.
-      intros m1; induction m1; cbn; intros m2 m3 eq; subst.
-      apply SO_base.
-      apply SO_step; apply suffix_of_prefixed.
-    Qed.
-
-    Theorem SuffixOf_iff : forall m1 m2, SuffixOf m1 m2 <-> exists m3, mod_app m3 m1 = m2.
-    Proof using.
-      intros m1 m2; split; [apply suffix_has_prefix | intros [m3 eq]].
-      apply has_prefix_is_suffix with (m3 := m3); auto.
-    Qed.
-
-    Lemma SuffixOf_modapp : forall m1 m2 m3, SuffixOf m1 m2 -> SuffixOf (mod_app m1 m3) (mod_app m2 m3).
-    Proof using.
-      intros m1 m2 m3; induction m3; cbn; intro sfx; auto.
-      apply SO_step; auto.
-    Qed.
-
-    Fixpoint extract_suffix (m1 m2 : mod) : option mod :=
-      if eqb m1 m2
-      then Some base
-      else if PeanoNat.Nat.ltb (mod_size m1) (mod_size m2)
-           then match m2 with
-                | base => None
-                | cons m2' p =>
-                    match extract_suffix m1 m2' with
-                    | Some m3 => Some (cons m3 p)
-                    | None => None
-                    end
-                end
-           else None.
-
-    Lemma extract_suffix_spec1 : forall m1 m2 m3, extract_suffix m1 m2 = Some m3 -> m2 = mod_app m1 m3.
-    Proof using.
-      intros m1 m2; revert m1; induction m2; cbn; intros m1 m3 eq.
-      - eq_bool; inversion eq; subst;  reflexivity.
-      - eq_bool; [inversion eq; clear eq|]; subst; cbn; [reflexivity|].
-        destruct (PeanoNat.Nat.leb_spec (mod_size m1) (mod_size m2)); [|inversion eq].
-        destruct (extract_suffix m1 m2) eqn:eq'; inversion eq; subst; clear eq.
-        apply IHm2 in eq'; subst; cbn; reflexivity.
-    Qed.
-
-    Lemma extract_suffix_self : forall m, extract_suffix m m = Some base.
-    Proof using.
-      intro m; induction m; cbn; eq_bool; reflexivity.
-    Qed.
-    
-    Lemma extract_suffix_spec2 : forall m1 m2, extract_suffix m1 (mod_app m1 m2) = Some m2.
-    Proof using.
-      intros m1 m2; revert m1; induction m2; cbn; intros m1; cbn; [apply extract_suffix_self|].
-      eq_bool; subst.
-      - exfalso. assert (mod_size m1 = mod_size (cons (mod_app m1 m2) p)) as eq_size by (f_equal; exact eq).
-        cbn in eq_size; rewrite mod_app_size in eq_size; lia.
-      - destruct (PeanoNat.Nat.leb_spec (mod_size m1) (mod_size (mod_app m1 m2))).
-        2: { rewrite mod_app_size in H0; exfalso; lia. }
-        rewrite IHm2; reflexivity.
-    Qed.
-
-    Theorem extract_suffix_spec : forall m1 m2 m3, extract_suffix m1 m2 = Some m3 <-> m2 = mod_app m1 m3.
-    Proof using.
-      intros m1 m2 m3; split; intro H0; [apply extract_suffix_spec1; auto | rewrite H0; apply extract_suffix_spec2].
-    Qed.
-
-    
-    Inductive PrefixOf : mod -> mod -> Prop :=
-    | PO_refl (m : mod) : PrefixOf m m
-    | PO_step {m1 m2 : mod} (pf : PrefixOf m1 m2) (p : PName)
-      : PrefixOf m1 (cons m2 p).
-
-    #[global] Instance PrefixOfRefl : Reflexive PrefixOf := PO_refl.
-
-    Lemma PrefixOf_base : forall m, PrefixOf base m.
-    Proof using.
-      intro m; induction m; constructor; auto.
-    Qed.
-
-    Lemma PrefixOf_app : forall m1 m2, PrefixOf m1 (mod_app m1 m2).
-    Proof using.
-      intros m1 m2; revert m1; induction m2; intro m1; cbn; constructor; auto.
-    Qed.
-
-    Lemma PrefixOf_peel : forall m1 m2, PrefixOf m1 m2 -> exists m2', m2 = mod_app m1 m2'.
-    Proof using.
-      intros m1 m2 pfx; induction pfx.
-      - exists base; reflexivity.
-      - destruct IHpfx as [m2' eq]; subst.
-        exists (cons m2' p); reflexivity.
-    Qed.
-
-    Lemma PrefixOf_antisym : forall m1 m2, PrefixOf m1 m2 -> PrefixOf m2 m1 -> m1 = m2.
-    Proof using.
-      intros m1 m2 pfx1 pfx2.
-      apply PrefixOf_peel in pfx1; destruct pfx1 as [m1' eq1].
-      apply PrefixOf_peel in pfx2; destruct pfx2 as [m2' eq2].
-      subst.
-      rewrite mod_app_assoc in eq2. apply mod_app_id_inv in eq2. apply mod_app_base_inv in eq2; destruct eq2; subst. cbn. reflexivity.
-    Qed.
-
-    #[global] Instance PrefixOfAntisym : Antisymmetric mod eq PrefixOf := PrefixOf_antisym.
-
-    Lemma PrefixOf_trans : forall m1 m2 m3, PrefixOf m1 m2 -> PrefixOf m2 m3 -> PrefixOf m1 m3.
-    Proof using.
-      intros m1 m2 m3 pfx1 pfx2; revert m1 pfx1; induction pfx2 as [m2 | m2 m3 pf IHpf p];
-        intros m1 pfx1.
-      - exact pfx1.
-      - apply PO_step; apply IHpf; exact pfx1.
-    Qed.
-
-    #[global] Instance PrefixOfTrans : Transitive PrefixOf := PrefixOf_trans.
-
-    Lemma PrefixOf_size : forall m1 m2, PrefixOf m1 m2 -> mod_size m1 <= mod_size m2.
-    Proof using.
-      intros m1 m2 pfx; induction pfx; cbn; lia.
-    Qed.
-
-    Lemma mod_app_mono_l : forall m1 m2 m3, PrefixOf m1 m2 -> PrefixOf (mod_app m3 m1) (mod_app m3 m2).
-    Proof using.
-      intros m1 m2 m3 pfx; revert m3; induction pfx; intro m3; [reflexivity|].
-      cbn; apply PO_step; apply IHpfx.
-    Qed.
-
-    Lemma extract_suffix_prefix : forall m1 m2 m3, extract_suffix m1 m2 = Some m3 -> PrefixOf m1 m2.
-    Proof using.
-      intros m1 m2; revert m1; induction m2; cbn; intros m1 m3 eq; eq_bool; try (inversion eq; subst; reflexivity; fail); subst.
-      destruct (PeanoNat.Nat.leb_spec (mod_size m1) (mod_size m2)); [| inversion eq].
-      destruct (extract_suffix m1 m2) eqn:eq'; inversion eq; subst; clear eq.
-      apply IHm2 in eq'. apply PO_step. exact eq'.
-    Qed.
-
-    Lemma prefix_extract_suffix : forall m1 m2, PrefixOf m1 m2 -> exists m3, extract_suffix m1 m2 = Some m3.
-    Proof using.
-      intros m1 m2 pfx.
-      destruct (PrefixOf_peel pfx) as [m3 eq]; subst.
-      exists m3; apply extract_suffix_spec2.
-    Qed.
-    
-    Fixpoint prefixb (m1 m2 : mod) : bool :=
-      if eqb m1 m2
-      then true
-      else match m2 with
-           | base => false
-           | cons m2' _ => prefixb m1 m2'
-           end.
-
-    Lemma prefixb_refl : forall m, prefixb m m = true.
-    Proof using.
-      intro m; destruct m; cbn; eq_bool; reflexivity.
-    Qed.
-
-    Lemma PrefixOf_prefixb : forall m1 m2, PrefixOf m1 m2 -> prefixb m1 m2 = true.
-    Proof using.
-      intros m1 m2 pfx; induction pfx; [apply prefixb_refl|].
-      cbn; eq_bool; subst; [reflexivity| assumption].
-    Qed.
-
-    Lemma prefixb_PrefixOf : forall m1 m2, prefixb m1 m2 = true -> PrefixOf m1 m2.
-    Proof using.
-      intros m1 m2; revert m1; induction m2 as [| m2' IHm2' p]; intros m1 eq; cbn in eq;
-        eq_bool; subst; try (constructor; auto; fail).
-      inversion eq.
-    Qed.
-
-    Theorem PrefixOf_dec : forall m1 m2, {PrefixOf m1 m2} + {~ PrefixOf m1 m2}.
-    Proof using H.
-      intros m1 m2; destruct (prefixb m1 m2) eqn:eq.
-      left; apply prefixb_PrefixOf; exact eq.
-      right; intro H'; apply PrefixOf_prefixb in H'; rewrite H' in eq; inversion eq.
-    Defined.
-
-    Theorem PrefixOf_app_mono : forall m1 {m2 m3}, PrefixOf m2 m3 -> PrefixOf (mod_app m1 m2) (mod_app m1 m3).
-    Proof using.
-      intros m1 m2 m3 pfx; revert m1; induction pfx as [m2 | m2 m3 pf IHpf p]; intro m1.
-      - reflexivity.
-      - cbn; constructor; apply IHpf.
-    Qed.
-
-    Fixpoint base_Prefix (m : mod) : PrefixOf base m :=
-      match m with
-      | base => PO_refl base
-      | cons m p => PO_step (base_Prefix m) p
-      end.
-
-    Fixpoint remove_Prefix (m1 m2 : mod) : option mod :=
-      if eqb m1 m2
-      then Some base
-      else match m2 with
-           | base => None
-           | cons m2' p =>
-               match remove_Prefix m1 m2' with
-               | None => None
-               | Some m => Some (cons m p)
-               end
-           end.
-
-    Lemma readd_remove_prefix : forall m1 m2 m3, remove_Prefix m1 m2 = Some m3 -> mod_app m1 m3 = m2.
-    Proof using.
-      intros m1 m2; revert m1; induction m2; intros m1 m3 eq; cbn in *;
-        eq_bool; subst; try (inversion eq; subst); cbn; try reflexivity.
-      destruct (remove_Prefix m1 m2) eqn:eq'; [|inversion eq].
-      inversion H1; subst; clear H1; cbn.
-      specialize (IHm2 m1 m eq'). rewrite IHm2. reflexivity.
-    Qed.
-
-    Lemma remove_all_mod : forall m, remove_Prefix m m = Some base.
-    Proof using.
-      intro m; destruct m; cbn; eq_bool; reflexivity.
-    Qed.
-
-    Lemma prefix_remove_Some : forall m1 m2, PrefixOf m1 m2 -> exists m, remove_Prefix m1 m2 = Some m.
-    Proof using.
-      intros m1 m2 pfx; induction pfx; cbn.
-      - exists base; apply remove_all_mod.
-      - eq_bool; subst; [exists base; reflexivity|].
-        destruct IHpfx as [m IHpfx].
-        exists (cons m p); rewrite IHpfx; reflexivity.
-    Qed.
-
-    Lemma remove_Some_prefix : forall m1 m2 m3, remove_Prefix m1 m2 = Some m3 -> PrefixOf m1 m2.
-    Proof using.
-      intros m1 m2; revert m1; induction m2; intros m1 m3 eq; cbn in eq;
-        eq_bool; subst; try (econstructor; eauto; fail).
-      inversion eq.
-      destruct (remove_Prefix m1 m2) eqn:eq'; inversion eq; subst.
-      specialize (IHm2 m1 m eq').
-      constructor; auto.
-    Qed.
-
-    Definition mod_eq_dec  : forall (m1 m2 : mod), {m1 = m2} + {m1 <> m2}.
-      refine (fix mod_eq_dec (m1 m2 : mod) :=
-                match m1, m2 with
-                | base, base => left eq_refl
-                | base, cons m2' p => right (fun eq => _)
-                | cons m1' p, base => right (fun eq => _)
-                | cons m1' p, cons m2' q =>
-                    match EqBool.eq_dec p q with
-                    | left eq_p_q =>
-                        match mod_eq_dec m1' m2' with
-                        | left eq_12 => left _
-                        | right neq_12 => right (fun eq => _)
-                        end
-                    | right neq_p_q => right (fun eq => _)
-                    end
-                end).
-      all: try (inversion eq; fail).
-      - rewrite eq_p_q; rewrite eq_12; reflexivity.
-      - inversion eq; subst; apply neq_12; reflexivity.
-      - inversion eq; subst; apply neq_p_q; reflexivity.
-    Defined.
-
-    Inductive PrefixOfT : mod -> mod -> Type :=
-    | POT_refl (m : mod) : PrefixOfT m m
-    | POT_step (m1 m2 : mod) (p : PName) (pfx : PrefixOfT m1 m2) : PrefixOfT m1 (cons m2 p).
-
-    Fixpoint PrefixOfT2Prefix {m1 m2 : mod} (pfx : PrefixOfT m1 m2) : PrefixOf m1 m2 :=
-      match pfx with
-      | POT_refl m => PO_refl m
-      | POT_step p pfx => PO_step (PrefixOfT2Prefix pfx) p
-      end.
-
-    Fixpoint base_PrefixT (m : mod) : PrefixOfT base m :=
-      match m with
-      | base => POT_refl base
-      | cons m p => POT_step p (base_PrefixT m)
-      end.
-
-    Fixpoint PrefixOfT_dec (m1 m2 : mod) : option (PrefixOfT m1 m2) :=
-      match mod_eq_dec m1 m2 with
-      | left e => ltac:(rewrite e; exact (Some (POT_refl m2)))
-      | right neq =>
-          match m2 with
-          | base =>
-              match m1 with
-              | base => Some (POT_refl base)
-              | _ => None
-              end
-          | cons m2' q =>
-              match PrefixOfT_dec m1 m2' with
-              | Some pfxt => Some (POT_step q pfxt)
-              | None => None
-              end
-          end
-      end.
-
-    Lemma Prefix2PrefixT : forall m1 m2, PrefixOf m1 m2 -> exists pfxt, PrefixOfT_dec m1 m2 = Some pfxt.
-    Proof using.
-      intros m1 m2 pfx; induction pfx; cbn.
-      - destruct m; cbn.
-        -- exists (POT_refl base); reflexivity.
-        -- destruct (EqBool.eq_dec p p) as [e|n]; [|destruct (n eq_refl)].
-           destruct (mod_eq_dec m m) as [e'|n]; [|destruct (n eq_refl)].
-           exists (POT_refl (cons m p)).
-           assert (e = eq_refl) by (apply (UIP_dec EqBool.eq_dec)).
-           assert (e' = eq_refl) by (apply (UIP_dec EqBool.eq_dec)).
-           rewrite H1; cbn. rewrite H0; cbn. reflexivity.
-      - destruct (mod_eq_dec m1 (cons m2 p)); subst; cbn.
-        -- exists (POT_refl (cons m2 p)); reflexivity.
-        -- destruct IHpfx as [pfxt IHpfx]. rewrite IHpfx.
-           eexists; reflexivity.
-    Qed.
-
-    Theorem PrefixT_equiv : forall m1 m2, PrefixOf m1 m2 <-> exists pfxt, PrefixOfT_dec m1 m2 = Some pfxt.
-    Proof using.
-      intros m1 m2; split; intro H0. exact (Prefix2PrefixT H0).
-      destruct H0 as [pfxt H0]. apply PrefixOfT2Prefix; exact pfxt.
-    Qed.
-
-    Fixpoint remove_PrefixT (m1 m2 : mod) (pfx : PrefixOfT m1 m2) :=
-      match pfx with
-      | POT_refl m => base
-      | POT_step p pfx' => cons (remove_PrefixT pfx') p
-      end.
-
-    Lemma Snm_false :forall n m, ~ (S ( n + m) = n).
-    Proof using.
-      intro n; induction n; cbn; intros m eq; inversion eq; subst.
-      apply IHn in H1; auto.
-    Qed.
-
-    Lemma Prefix_modapp_inv : forall m1 m2, PrefixOf (mod_app m1 m2) m1 -> m2 = base.
-    Proof using.
-      intro m1; induction m1; intros m2 pfx.
-      - rewrite mod_base_app in pfx; inversion pfx; subst; reflexivity.
-      - inversion pfx; subst.
-        -- clear IHm1 pfx; induction m2; [reflexivity| cbn in *].
-           inversion H2; subst.
-           assert (mod_size (mod_app (cons m1 p) m2) = mod_size m1) as eq by (f_equal; exact H1).
-           rewrite mod_app_size in eq; cbn in eq.
-           apply Snm_false in eq; exfalso; auto.
-        -- assert (cons m1 p = mod_app m1 (cons base p)) as eq by reflexivity; rewrite eq in pf.
-           rewrite mod_app_assoc in pf. apply IHm1 in pf.
-           clear eq pfx IHm1 m1.
-           exfalso; induction m2; cbn in pf; inversion pf.
-    Qed.           
-    
-    Lemma PrefixT_modapp_inv : forall m1 m2, PrefixOfT (mod_app m1 m2) m1 -> m2 = base.
-    Proof using.
-      intro m1; induction m1; intros m2 pfx.
-      - rewrite mod_base_app in pfx; inversion pfx; subst; reflexivity.
-      - inversion pfx; subst.
-        -- clear IHm1 pfx; induction m2; [reflexivity| cbn in *].
-           inversion H2; subst.
-           assert (mod_size (mod_app (cons m1 p) m2) = mod_size m1) as eq by (f_equal; exact H1).
-           rewrite mod_app_size in eq; cbn in eq.
-           apply Snm_false in eq; exfalso; auto.
-        -- assert (cons m1 p = mod_app m1 (cons base p)) as eq by reflexivity; rewrite eq in pfx0.
-           rewrite mod_app_assoc in pfx0. apply IHm1 in pfx0.
-           clear eq pfx IHm1 m1.
-           exfalso; induction m2; cbn in pfx0; inversion pfx0.
-    Qed.           
-    
-    Lemma PrefixT_cons_inv : forall m p, PrefixOfT (cons m p) m -> False.
-    Proof using.
-      intros m p.
-      assert (cons m p = mod_app m (cons base p)) as eq by reflexivity; rewrite eq; intro pfx.
-      apply PrefixT_modapp_inv in pfx.
-      inversion pfx.
-    Qed.
-
-    Lemma remove_PrefixT_ext : forall (m1 m2 : mod) (pfx1 pfx2 : PrefixOfT m1 m2),
-        remove_PrefixT pfx1 = remove_PrefixT pfx2.
-    Proof using.
-      intros m1 m2; revert m1; induction m2; intros m1 pfx1 pfx2.
-      - inversion pfx1; subst.
-        dependent destruction pfx1; dependent destruction pfx2; reflexivity.
-      - dependent destruction pfx1; dependent destruction pfx2; cbn; auto.
-        -- exfalso; apply PrefixT_cons_inv in pfx2; auto.
-        -- exfalso; apply PrefixT_cons_inv in pfx1; auto.
-        -- rewrite IHm2 with (pfx2 := pfx2); reflexivity.
-    Qed.
-
-    Program Fixpoint PrefixT_peel (m1 m2 : mod) : PrefixOfT m1 (mod_app m1 m2) :=
-      match m2 with
-      | base => POT_refl m1
-      | cons m2 p => POT_step p (PrefixT_peel m1 m2)
-      end.
-    
-    Lemma remove_PrefixT_app : forall (m1 m2 : mod) (pfx : PrefixOfT m1 (mod_app m1 m2)),
-        remove_PrefixT pfx = m2.
-    Proof using.
-      intros m1 m2 pfx.
-      rewrite remove_PrefixT_ext with (pfx2 := PrefixT_peel m1 m2); clear pfx.
-      revert m1; induction m2; intro m1; cbn; auto.
-      rewrite IHm2; reflexivity.
-    Qed.
-    
-    Definition remove_Prefix' : forall (m1 m2 : mod) (pfx : PrefixOf m1 m2), mod.
-      refine (fix remove_Prefix' m1 m2 pfx :=
-                match mod_eq_dec m1 m2 with
-                | left _ => base
-                | right neq =>
-                    (match m2 as a return a = m2 -> mod with
-                     | base => fun eq => False_rect mod _
-                     | cons m2' p =>
-                         fun eq => cons (@remove_Prefix' m1 m2' _) p
-                     end) eq_refl
-                end).
-      - rewrite <- eq in pfx. inversion pfx; subst. destruct (neq eq_refl).
-      - subst; inversion pfx; subst; [exfalso; apply neq; reflexivity | exact pf].
-    Defined.
-
-    Fixpoint remove_list_prefix  {A : Type} `{eqdec : EqBool A} (l1 l2 : list A) : option (list A) :=
-      match l1, l2 with
-      | [], _ => Some l2
-      | (_ :: _), [] => None
-      | (x :: xs), (y :: ys) => if eqb x y then remove_list_prefix xs ys else None
-      end.
-
-    Lemma remove_list_prefix_nil : forall {A : Type} `{eqdec :EqBool A} (l : list A), remove_list_prefix l l = Some [].
-    Proof using.
-      intros A eqdec l; induction l; cbn. reflexivity.
-      eq_bool; auto.
-    Qed.
-
-    Lemma remove_list_prefix_front : forall {A : Type} `{eqbool : EqBool A} (l1 l2 l3 l4 : list A),
-        remove_list_prefix l1 l2 = Some l3 ->
-        remove_list_prefix l1 (l2 ++ l4) = Some (l3 ++ l4).
-    Proof using.
-      intros A eqbool l1; induction l1; intros l2 l3 l4 eq; cbn in *.
-      - inversion eq; subst; reflexivity.
-      - destruct l2; cbn in *. inversion eq.
-        eq_bool; subst.
-        -- apply IHl1; auto.
-        -- inversion eq.
-    Qed.
-
-    Lemma remove_list_PrefixOf : forall (m1 m2 : mod), PrefixOf m1 m2 -> exists l, remove_list_prefix (mod2list m1) (mod2list m2) = Some l.
-    Proof using.
-      intros m1 m2 pfx; induction pfx; cbn.
-      - exists []; apply remove_list_prefix_nil.
-      - destruct IHpfx as [l' eq].
-        exists (l' ++ [p]). apply remove_list_prefix_front. exact eq.
-    Qed.
-    
-    
-    (* Lemma remove_prefix_prime : forall (m1 m2 : mod) (pfx : PrefixOf m1 m2), *)
-    (*     remove_Prefix m1 m2 = Some (remove_Prefix' pfx). *)
-    (* Proof using. *)
-    (*   intros m1 m2; revert m1; induction m2; intros m1; intro pfx; cbn; eq_bool; subst; *)
-    (*     try (reflexivity). *)
-    (*   - inversion pfx; subst. exfalso; apply neq; reflexivity. *)
-    (*   - destruct (mod_eq_dec (cons m2 p) (cons m2 p)) as [e' | n]; [|destruct (n eq_refl)]. *)
-    (*     reflexivity. *)
-    (*   - destruct (mod_eq_dec m1 (cons m2 p)) as [e' | n]; [destruct (neq e')|]. *)
-    (*     inversion pfx; subst. destruct (n eq_refl). *)
-
-    (* Equations remove_Prefix' (m1 m2 : mod) (pfx : PrefixOf m1 m2) : mod := *)
-    (*   { *)
-    (*     remove_Prefix' m1 m2 pfx with dec_eq m1 m2 => { *)
-    (*       remove_Prefix' m1 m2 pfx (left _) := base; *)
-    (*       remove_Prefix' base base (PO_refl _) (right neq) with (neq eq_refl) => { }; *)
-    (*       remove_Prefix' m1 (cons m2 p) (PO_step pf' p) (right neq) := cons (remove_Prefix' m1 m2 pf')     *)
-    (*     } *)
-    (*   }. *)
-    
-  End Modality.
-
 
   Section Contexts.
 
@@ -753,7 +108,6 @@ Section CorpsSyntax.
       - apply ConsTowerOn_antirefl with (m := m); exact cot.
       - apply IHpfxt. apply ConsTower_reduce with (p := p). exact cot.
     Defined.
-
     
     Lemma UIprefixT : forall m1 m2 (pfx1 pfx2 : PrefixOfT m1 m2), pfx1 = pfx2.
     Proof using H PName.
@@ -810,8 +164,8 @@ Section CorpsSyntax.
               | Some pfx =>
                   Some ({|
                         vars n :=  vars Γ n;
-                        locks n := @remove_PrefixT m (locks Γ n) (prefixT_prefix_trans pfx (@locks_mono Γ 0 n ltac:(lia)));
-                        all_locks := @remove_PrefixT m (all_locks Γ) (prefixT_prefix_trans pfx (@locks_bound Γ 0));
+                        locks n := @remove_PrefixT PName m (locks Γ n) (prefixT_prefix_trans pfx (@locks_mono Γ 0 n ltac:(lia)));
+                        all_locks := @remove_PrefixT PName m (all_locks Γ) (prefixT_prefix_trans pfx (@locks_bound Γ 0));
                         locks_mono := _;
                         locks_bound := _;
                       |})
@@ -820,44 +174,6 @@ Section CorpsSyntax.
       - intros n; apply remove_prefix_mono; apply (locks_bound Γ).
     Defined.
 
-    Lemma cons_self_no : forall m p, m <> cons m p.
-    Proof using.
-      intro m; induction m; cbn; intros q eq; inversion eq; subst.
-      apply IHm in H1; auto.
-    Qed.
-
-    Lemma cons_app_self_no1 : forall m1 m2 p, m1 <> cons (mod_app m1 m2) p.
-    Proof using.
-      intros m1 m2 p eq. assert (m1 = mod_app m1 (cons m2 p)) as H0 by exact eq; apply mod_app_id_inv in H0.
-      inversion H0.
-    Qed.
-
-    Lemma mod_app_front : forall m1 m2 m3, mod_app m1 m2 = mod_app m1 m3 -> m2 = m3.
-    Proof using.
-      intros m1 m2; revert m1; induction m2; cbn; intros m1 m3 eq.
-      - apply mod_app_id_inv in eq; symmetry; exact eq.
-      - destruct m3; cbn in eq. symmetry in eq; apply cons_app_self_no1 in eq; destruct eq.
-        inversion eq; subst. apply IHm2 in H1; subst. reflexivity.
-    Qed.
-
-    Lemma mod_app_prefix : forall m1 m2 m3, PrefixOf (mod_app m1 m2) (mod_app m1 m3) -> PrefixOf m2 m3.
-    Proof using.
-      intros m1 m2 m3; revert m1 m2; induction m3; intros m1 m2 pfx.
-      - apply Prefix_modapp_inv in pfx; subst; reflexivity.
-      - inversion pfx; subst.
-        2: { specialize (IHm3 _ _ pf); apply PO_step; exact IHm3. }
-        assert (mod_app m1 m2 = mod_app m1 (cons m3 p)) as H0 by (exact H2); apply mod_app_front in H0; subst.
-        reflexivity.
-    Qed.
-
-    Lemma common_suffix : forall m1 m2 m3, PrefixOf m1 m3 -> PrefixOf m2 m3 -> PrefixOf m1 m2 \/ PrefixOf m2 m1.
-    Proof using.
-      intros m1 m2 m3; revert m1 m2; induction m3; intros m1 m2 pfx1 pfx2.
-      - inversion pfx1; inversion pfx2; subst; left; reflexivity.
-      - inversion pfx1; subst; [right; exact pfx2|].
-        inversion pfx2; subst; [left; exact pfx1|].
-        apply IHm3; auto.
-    Qed.
 
     (* Program Definition replace_lock_prefix (Γ : Ctxt) (m1 m2 : mod) : option Ctxt := *)
     (*   match extract_suffix m1 (all_locks Γ) with *)
@@ -1014,9 +330,9 @@ Section CorpsSyntax.
     | efql (e : expr) (* ex falso quod libet; exfalso is taken by coq *)
     | lam (t : type) (e : expr)
     | appE (e1 e2 : expr)
-    | send (e : expr) (p : PName) (Δ : FiniteCtxt) (q : PName)
-    | up (e : expr) (p : PName) (Δ : FiniteCtxt)
-    | down (e : expr) (p : PName) (Δ : FiniteCtxt).
+    | send (e : expr) (seen : nat) (m : mod) (p : PName) (q : PName)
+    | up (e : expr)(seen : nat) (m : mod) (p : PName)
+    | down (e : expr) (seen : nat) (m : mod) (p : PName).
 
     Fixpoint expr_eqb (e1 e2 : expr) : bool :=
       match e1, e2 with
@@ -1034,9 +350,12 @@ Section CorpsSyntax.
       | efql e1, efql e2 => expr_eqb e1 e2
       | lam t1 e1, lam t2 e2 => eqb t1 t2 && expr_eqb e1 e2
       | appE e11 e12, appE e21 e22 => expr_eqb e11 e21 && expr_eqb e12 e22
-      | send e1 p1 Δ1 q1, send e2 p2 Δ2 q2 => expr_eqb e1 e2 && eqb Δ1 Δ2 && eqb p1 p2 && eqb q1 q2
-      | up e1 p Δ1, up e2 q Δ2 => expr_eqb e1 e2 && eqb Δ1 Δ2 && eqb p q
-      | down e1 p Δ1, down e2 q Δ2 => expr_eqb e1 e2 && eqb Δ1 Δ2 && eqb p q
+      | send e1 seen1 m1 p1 q1, send e2 seen2 m2 p2 q2 =>
+          expr_eqb e1 e2 && eqb seen1 seen2 && eqb m1 m2&& eqb p1 p2 && eqb q1 q2
+      | up e1 seen1 m1 p1, up e2 seen2 m2 p2 =>
+          expr_eqb e1 e2 && eqb seen1 seen2 && eqb m1 m2 && eqb p1 p2
+      | down e1 seen1 m1 p1, down e2 seen2 m2 p2 =>
+          expr_eqb e1 e2 && eqb seen1 seen2 && eqb m1 m2 && eqb p1 p2
       | _, _ => false 
       end.
 
@@ -1133,9 +452,9 @@ Section CorpsSyntax.
       | efql e => efql (ren e ξ)
       | lam t e => lam t (ren e (renup ξ))
       | appE e1 e2 => appE (ren e1 ξ) (ren e2 ξ)
-      | send e p Δ q => send (ren e ξ) p Δ q
-      | up e p Δ => up (ren e ξ) p Δ
-      | down e p Δ => down (ren e ξ) p Δ
+      | send e seen m p q => send (ren e ξ) seen m p q
+      | up e seen m p => up (ren e ξ) seen m p
+      | down e seen m p => down (ren e ξ) seen m p
       end.
     
     Lemma ren_ext : forall (ξ1 ξ2 : renaming),
@@ -1162,6 +481,7 @@ Section CorpsSyntax.
           | [|- ?a = ?a ] => reflexivity
           | [|- context[id_renaming _]] => unfold id_renaming; cbn
           | [ H : ren ?e id_renaming = ?e |- context[ren ?e id_renaming]] => rewrite H
+          | [ H : ren ?e id_renaming = ?e |- context[ren ?e (fun x => x)]] => unfold id_renaming in H; rewrite H
           | [|- context[ren ?e (renup id_renaming)]] =>
               rewrite (ren_ext (renup id_renaming) id_renaming renup_id e)
           end.
@@ -1298,7 +618,15 @@ Section CorpsSyntax.
       rewrite id_below; [reflexivity|].
       lia.
     Qed.
-    
+
+    Definition option_bind {A B : Type} (x : option A) (f : A -> option B) : option B :=
+      match x with
+      | Some a => f a
+      | None => None
+      end.
+
+    #[local] Notation "x >>= f" := (option_bind x f) (at level 10).
+
     Fixpoint subst (e : expr) (σ : substitution) : expr :=
       match e with
       | var x => σ x
@@ -1315,10 +643,9 @@ Section CorpsSyntax.
       | efql e => efql (subst e σ)
       | lam t e => lam t (subst e (substup σ))
       | appE e1 e2 => appE (subst e1 σ) (subst e2 σ)
-      (* | send e p Δ q => send (subst e (substup_many σ (FiniteCtxtSize Δ))) p Δ q *)
-      | send e p Δ q => send (subst e σ) p Δ q
-      | up e p Δ => up (subst e σ) p Δ
-      | down e p Δ => down (subst e σ) p Δ
+      | send e seen m p q => send (subst e σ) seen m p q
+      | up e seen m p => up (subst e σ) seen m p
+      | down e seen m p => down (subst e σ) seen m p
       end.
 
     Lemma subst_ext : forall σ1 σ2,
@@ -1451,12 +778,12 @@ Section CorpsSyntax.
     | lam_ca (t : type) {e : expr} {n : nat} (pf : closed_above e (S n)) : closed_above (lam t e) n
     | app_ca {e1 e2 : expr} {n : nat} (pf1 : closed_above e1 n) (pf2 : closed_above e2 n)
       : closed_above (appE e1 e2) n
-    | send_ca {e : expr} (Δ : FiniteCtxt) (p q : PName) {n : nat} (pf : closed_above e n)
-      : closed_above (send e p Δ q) n
-    | up_ca {e : expr} (p : PName) (Δ : FiniteCtxt) {n : nat} (pf : closed_above e n)
-      : closed_above (up e p Δ) n
-    | down_ca {e : expr} (p : PName) (Δ : FiniteCtxt) {n : nat} (pf : closed_above e n)
-      : closed_above (down e p Δ) n.
+    | send_ca {e : expr} (seen : nat) (m : mod) (p q : PName) {n : nat} (pf : closed_above e n)
+      : closed_above (send e seen m p q) n
+    | up_ca {e : expr} (seen : nat) (m : mod) (p : PName) {n : nat} (pf : closed_above e n)
+      : closed_above (up e seen m p) n
+    | down_ca {e : expr} (seen : nat) (m : mod) (p : PName) {n : nat} (pf : closed_above e n)
+      : closed_above (down e seen m p) n.
 
     Fixpoint closed_aboveb (e : expr) (n : nat) : bool :=
       match e with
@@ -1473,14 +800,14 @@ Section CorpsSyntax.
       | efql e => closed_aboveb e n
       | lam t e => closed_aboveb e (S n)
       | appE e1 e2 => closed_aboveb e1 n && closed_aboveb e2 n
-      | send e p Δ q => closed_aboveb e n
-      | up e p Δ => closed_aboveb e n
-      | down e p Δ => closed_aboveb e n
+      | send e seen m p q => closed_aboveb e n
+      | up e seen m p => closed_aboveb e n
+      | down e seen m p => closed_aboveb e n
       end.
 
     Lemma closed_aboveb_spec1 : forall e n, closed_aboveb e n = true -> closed_above e n.
     Proof using.
-      intro e; induction e; cbn; intros m clsdb;
+      intro e; induction e; cbn; intros n' clsdb;
         repeat match goal with
           | [ H : _ && _ = true |- _ ] => apply andb_prop in H; destruct H
           end;
@@ -1660,9 +987,9 @@ Section CorpsSyntax.
       | efql e => min_closure e
       | lam t e => pred (min_closure e)
       | appE e1 e2 => max (min_closure e1) (min_closure e2)
-      | send e p Δ q => min_closure e
-      | up e p Δ => min_closure e
-      | down e p Δ => min_closure e
+      | send e seen m p q => min_closure e
+      | up e seen m p => min_closure e
+      | down e seen m p => min_closure e
       end.
 
     Theorem closed_above_min : forall e, closed_above e (min_closure e).
@@ -1700,133 +1027,6 @@ Section CorpsSyntax.
         -- rewrite eq_locks; reflexivity.
     Qed.
 
-    Fixpoint change_prefix_t {m1 m2 : mod} (pfx1 : PrefixOfT m1 m2) (m3 : mod) : mod :=
-      match pfx1 with
-      | POT_refl _ => m3
-      | POT_step p pfx => cons (change_prefix_t pfx m3) p
-      end.
-
-    Lemma change_prefix_t_prefix : forall {m1 m2 : mod} (pfx : PrefixOfT m1 m2) (m3 : mod),
-        PrefixOf m3 (change_prefix_t pfx m3).
-    Proof using.
-      intros m1 m2 pfx; dependent induction pfx; intro m3; cbn.
-      reflexivity.
-      apply PO_step; apply IHpfx.
-    Qed.
-
-    Fixpoint PrefixT_app (m1 m2 : mod) : PrefixOfT m1 (mod_app m1 m2) :=
-      match m2 with
-      | base => POT_refl m1
-      | cons m2' p => POT_step p (PrefixT_app m1 m2')
-      end.
-
-    Lemma change_prefix_t_spec : forall m1 m2 m3, change_prefix_t (PrefixT_app m1 m2) m3 = mod_app m3 m2.
-    Proof using.
-      intros m1 m2; revert m1; induction m2; intros m1 m3; cbn.
-      reflexivity.
-      f_equal; apply IHm2.
-    Qed.
-
-    Fixpoint change_prefix (m1 m2 m3 : mod) : option mod :=
-      if eqb m1 m2
-      then Some m3
-      else match m2 with
-           | base => None
-           | cons m2' p =>
-               match change_prefix m1 m2' m3 with
-               | None => None
-               | Some m => Some (cons m p)
-               end
-           end.
-
-    Theorem change_prefix_of_prefix : forall (m1 m2 m3 : mod),
-        PrefixOf m1 m2 ->
-        change_prefix m1 m2 m3 <> None.
-    Proof using.
-      intros m1 m2; revert m1; induction m2; intros m1 m3 pfx; cbn; eq_bool; subst; try discriminate.
-      - inversion pfx; subst; exfalso; apply neq; reflexivity.
-      - inversion pfx; subst; [exfalso; apply neq; reflexivity|].
-        destruct (change_prefix m1 m2 m3) eqn:eq; [discriminate|].
-        exfalso; apply IHm2 with (m1 := m1) (m3 := m3); auto.
-    Qed.
-
-    Lemma cons_prefix : forall m1 m2 p, PrefixOf (cons m1 p) m2 -> PrefixOf m1 m2.
-    Proof using H PName.
-      intros m1 m2 p pfx; dependent induction pfx.
-      - apply PO_step; reflexivity.
-      - specialize (IHpfx H m1 p eq_refl); apply PO_step; apply IHpfx.
-    Qed.
-    
-    Lemma extended_suffix_not_prefix : forall m1 m2 p, PrefixOf m1 m2 -> ~ (PrefixOf (cons m2 p) m1).
-    Proof using H PName.
-      intros m1; induction m1; intros m2 q pfx1 pfx2.
-      - inversion pfx2.
-      - inversion pfx2; subst.
-        apply IHm1 with (m2 := m1) (p := p); [reflexivity | exact pfx1].
-        apply (IHm1 m2 q); [apply cons_prefix with (p := p); exact pfx1 | exact pf].
-    Qed.
-
-    Theorem change_prefix_of_suffix : forall (m1 m2 m3 : mod),
-        PrefixOf m2 m1 ->
-        change_prefix m1 m2 m3 = None \/ m1 = m2.
-    Proof using.
-      intros m1 m2; revert m1; induction m2; intros m1 m3 pfx; cbn; eq_bool; subst; auto.
-      left.
-      assert (PrefixOf m2 m1). clear IHm2 m3 e neq; dependent induction pfx. apply PO_step; apply PO_refl.
-      specialize (IHpfx H m2 p eq_refl). apply PO_step; exact IHpfx.
-      destruct (IHm2 m1 m3 H0); [rewrite H1; reflexivity| subst].
-      apply extended_suffix_not_prefix  with (p := p) in pfx.
-      exfalso; apply pfx; reflexivity.
-    Qed.      
-
-    Lemma change_prefix_of_prefix' : forall (m1 m2 m2' m3 m4 m4' : mod),
-        change_prefix m1 m2 m3 = Some m4 ->
-        change_prefix m1 m2' m3 = Some m4' ->
-        PrefixOf m2 m2' ->
-        PrefixOf m4 m4'.
-    Proof using.
-      intros m1 m2 m2' m3 m4 m4' H0 H1 pfx2; revert m1 m3 m4 m4' H0 H1; dependent induction pfx2;
-        [| rename m1 into m5; rename m2 into m5']; intros m1 m3 m4 m4' eq0 eq1.
-      - rewrite eq0 in eq1; inversion eq1; reflexivity.
-      - cbn in eq1; cbn in eq0; eq_bool; subst.
-        -- inversion eq1; subst; clear eq1.
-           destruct (change_prefix_of_suffix m4'  (PO_step pfx2 p)); subst.
-           rewrite H0 in eq0; inversion eq0.
-           cbn in eq0; eq_bool; inversion eq0; subst; reflexivity.
-        -- destruct (change_prefix m1 m5' m3) eqn:eq2; inversion eq1; subst; clear eq1.
-           apply PO_step. apply IHpfx2 with (m1 := m1)(m3 := m3); auto.
-    Qed.
-
-    Lemma prefix_of_change_prefix : forall (m1 m2 m3 m4 m5 : mod),
-        change_prefix m1 m2 m3 = Some m4 ->
-        PrefixOf m5 m3 ->
-        PrefixOf m5 m4.
-    Proof using.
-      intros m1 m2; revert m1; induction m2; cbn; intros m1 m3 m4 m5 eq pfx; eq_bool; subst;
-        try (inversion eq; subst; auto; fail).
-      destruct (change_prefix m1 m2 m3) eqn:eq'; inversion eq; subst; clear eq.
-      apply PO_step; eapply IHm2; eauto.
-    Qed.
-
-    Lemma only_prefixes_changable : forall m1 m2 m3 m4,
-        change_prefix m1 m2 m3 = Some m4 ->
-        PrefixOf m1 m2.
-    Proof using.
-      intros m1 m2; revert m1; induction m2; cbn; intros m1 m3 m4 eq;
-        eq_bool; subst; inversion eq; subst; clear eq; try reflexivity.
-      destruct (change_prefix m1 m2 m3) eqn: eq; inversion H1; subst; clear H1.
-      apply PO_step; eapply IHm2; eauto.
-    Qed.
-
-    Lemma prefix_changed_to_prefix : forall m1 m2 m3 m4,
-        change_prefix m1 m2 m3 = Some m4 ->
-        PrefixOf m3 m4.
-    Proof using.
-      intros m1 m2; revert m1; induction m2; cbn; intros m1 m3 m4 eq;
-        eq_bool; subst; inversion eq; subst; clear eq; try reflexivity.
-      destruct (change_prefix m1 m2 m3) eqn: eq; inversion H1; subst; clear H1.
-      apply PO_step; eapply IHm2; eauto.
-    Qed.
     
     Program Definition change_lock (Γ : Ctxt) (m1 m2 : mod) (inv : forall n, PrefixOf m1 (locks Γ n) \/ PrefixOf (locks Γ n) m2) :=
       {|
@@ -1868,7 +1068,84 @@ Section CorpsSyntax.
         apply prefix_changed_to_prefix in eq1; transitivity m2; auto.
       - apply locks_bound.
     Qed.
+
+    Lemma inv_ext : forall  (Γ Δ : Ctxt) (m1 m2 : mod),
+        ctxt_equiv Γ Δ ->
+        (forall n, PrefixOf m1 (locks Γ n) \/ PrefixOf (locks Γ n) m2) ->
+        forall n, PrefixOf m1 (locks Δ n) \/ PrefixOf (locks Δ n) m2.
+    Proof using.
+      intros Γ Δ m1 m2 [vars_equiv [locks_equiv al_eqv]] Γ_inv n.
+      destruct (Γ_inv n) as [pfx | pfx]; [left | right]; rewrite <- locks_equiv; auto.
+    Qed.
+      
+    Lemma change_lock_inv_ext : forall {Γ : Ctxt} {m1 m2 : mod} (inv1 inv2 : forall n, PrefixOf m1 (locks Γ n) \/ PrefixOf (locks Γ n) m2),
+        ctxt_equiv (change_lock Γ inv1) (change_lock Γ inv2).
+    Proof using.
+      intros Γ m1 m2 inv1 inv2; destruct Γ; cbn in *.
+      split; [| split]; try intro x; cbn; auto.
+    Qed.
+
+    Lemma change_lock_ctxt_ext : forall {Γ Δ : Ctxt} {m1 m2 : mod} (inv : forall n, PrefixOf m1 (locks Γ n) \/ PrefixOf (locks Γ n) m2)
+                                   (eqv : ctxt_equiv Γ Δ),
+        ctxt_equiv (change_lock Γ inv) (change_lock Δ (inv_ext eqv inv)).
+    Proof using.
+      intros Γ Δ m1 m2 inv [vars_eqv [locks_eqv al_eqv]].
+      split; [| split]; try intro x; cbn; auto.
+      rewrite locks_eqv; reflexivity.
+      rewrite al_eqv; reflexivity.
+    Qed.
+
+    Lemma change_lock_ext : forall {Γ Δ : Ctxt} {m1 m2 : mod} (inv1 : forall n, PrefixOf m1 (locks Γ n) \/ PrefixOf (locks Γ n) m2)
+                              (inv2 : forall n, PrefixOf m1 (locks Δ n) \/ PrefixOf (locks Δ n) m2),
+        ctxt_equiv Γ Δ ->
+        ctxt_equiv (change_lock Γ inv1) (change_lock Δ inv2).
+    Proof using.
+      intros Γ Δ m1 m2 inv1 inv2 eqv;
+        transitivity (change_lock Δ (inv_ext eqv inv1)); [apply change_lock_ctxt_ext | apply change_lock_inv_ext].
+    Qed.
     
+    Theorem change_lock_inv_send : forall (Γ : Ctxt) (m : mod) (p q : PName) (seen : nat),
+        locks Γ seen = cons m p ->
+        forall n, PrefixOf (cons m p) (locks Γ n)  \/ PrefixOf (locks Γ n) (cons m q).
+    Proof using.
+      intros Γ m p q seen seen_cons n.
+      destruct (PeanoNat.Nat.leb_spec n seen).
+      pose proof (locks_mono Γ H0) as prefix_n_seen; dependent destruction prefix_n_seen.
+      - left; rewrite x; rewrite seen_cons; reflexivity.
+      - rewrite seen_cons in x; inversion x; subst; clear x.
+        right. apply PO_step. exact prefix_n_seen.
+      - left; transitivity (locks Γ seen). rewrite seen_cons; reflexivity.
+        apply locks_mono; apply PeanoNat.Nat.lt_le_incl; exact H0.
+    Qed.           
+
+    Theorem change_lock_inv_up : forall (Γ : Ctxt) (m : mod) (p : PName) (seen : nat),
+        locks Γ seen = m ->
+        forall n, PrefixOf m (locks Γ n) \/ PrefixOf (locks Γ n) (cons m p).
+    Proof using.
+      intros Γ m p seen seen_cons n.
+      destruct (PeanoNat.Nat.leb_spec n seen) as [n_le_seen | seen_lt_n].
+      - pose proof (locks_mono Γ n_le_seen) as prefix_n_seen; dependent destruction prefix_n_seen.
+        -- left; rewrite <- seen_cons; rewrite <- x; reflexivity.
+        -- rewrite seen_cons in x; inversion x; subst.
+           right; do 2 apply PO_step; exact prefix_n_seen.
+      - left; transitivity (locks Γ seen). rewrite seen_cons; reflexivity.
+        apply locks_mono; apply PeanoNat.Nat.lt_le_incl; exact seen_lt_n.
+    Qed.
+
+    Theorem change_lock_inv_down : forall (Γ : Ctxt) (m : mod) (p : PName) (seen : nat),
+        locks Γ seen = cons m p ->
+        forall n, PrefixOf (cons m p) (locks Γ n) \/ PrefixOf (locks Γ n) m.
+    Proof using.
+      intros Γ m p seen locks_seen n.
+      destruct (PeanoNat.Nat.leb_spec n seen) as [n_le_seen | seen_lt_n].
+      - pose proof (locks_mono Γ n_le_seen) as prefix_n_seen; dependent destruction prefix_n_seen.
+        -- left; rewrite <- locks_seen; rewrite <- x; reflexivity.
+        -- rewrite locks_seen in x; inversion x; subst; clear x.
+           right; auto.
+      - left; transitivity (locks Γ seen). rewrite locks_seen; reflexivity.
+        apply locks_mono; apply PeanoNat.Nat.lt_le_incl; exact seen_lt_n.
+    Qed.    
+
   End Lockpointer.
 
   
